\documentclass{article}
\usepackage{amsmath}

\begin{document}
    \section*{Problem 1 Answer}
    The future value $FV$ of two bonds at horizon:
    \begin{equation}
        \begin{aligned}
            FV &= FV_{1} + FV_{2}\\
            &=P_{1}(1+y)^{D} + P_{2}(1+y)^{D} \\
        \end{aligned}
        \label{fv}
    \end{equation}
    where $P_{1}$ is the price of the first bond; $P_{2}$ is the price of the second bond. $D$ is the horizon. $y$ is the interest rate.\\
    For each bond, its price is
    \begin{equation}
        \label{pv}
        P = \sum_{i=1}^{n} \frac{C}{(1+y)^i} + \frac{F}{(1+y)^{n}}
    \end{equation}
    where $n$ is the term to maturity. C is the coupon payment. $F$ is par value of the bond.\\
    Use $P$ in (\ref{pv}) to substitute $P_{1}$ and $P_{2}$ in (\ref{fv}):

    \begin{equation*}
        \begin{aligned}
            FV &= \left(\sum_{i=1}^{n_{1}} \frac{C_{1}}{(1+y)^{i}} + \frac{F_{1}}{(1+y)^{n_{1}}}\right)(1+y)^{D} + \left(\sum_{i=1}^{n_{2}} \frac{C_{2}}{(1+y)^{i}} + \frac{F_{2}}{(1+y)^{n_{2}}}\right)(1+y)^{D} \\
            &= \sum_{i=1}^{n_{1}} C_{1}(1+y)^{D-i} + F_{1}(1+y)^{D-n_{1}} + \sum_{i=1}^{n_{2}} C_{2}(1+y)^{D-i} + F_{2}(1+y)^{D-n_{2}}
        \end{aligned}
    \end{equation*}
    At horizon,
    \begin{equation}
        \label{require 1}
        \frac{\partial FV}{\partial y} = \frac{\partial FV_{1}}{\partial y}=\frac{\partial FV_{2}}{\partial y}=0
    \end{equation}
    The partial derivative $FV$ over $y$:
    \begin{equation}
        \label{partial 1}
        \begin{aligned}
            \frac{\partial FV}{\partial y} &= \sum_{i=1}^{n_{1}} (D-i)C_{1}(1+y)^{D-i-1} + (D-n_{1})F_{1}(1+y)^{D-n_{1}-1} \\& +\sum_{i=1}^{n_{2}} (D-i)C_{2}(1+y)^{D-i-1} + (D-n_{2})F_{2}(1+y)^{D-n_{2}-1}
        \end{aligned}
    \end{equation}
    According to (\ref{require 1}) and (\ref{partial 1}):
    \begin{equation}
        \begin{aligned}
            \sum_{i=1}^{n_{1}} (D-i)C_{1}(1+y)^{D-i-1} + (D-n_{1})F_{1}(1+y)^{D-n_{1}-1} \\
            +\sum_{i=1}^{n_{2}} (D-i)C_{2}(1+y)^{D-i-1} + (D-n_{2})F_{2}(1+y)^{D-n_{2}-1} &= 0\\
            (1+y)^{D-1}\left[\sum_{i=1}^{n_{1}}\frac{(D-i)C_{1}}{(1+y)^{i}} + \frac{(D-n_{1})F_{1}}{(1+y)^{n_{1}}} + \sum_{i=1}^{n_{2}}\frac{(D-i)C_{2}}{(1+y)^{i}} + \frac{(D-n_{2})F_{2}}{(1+y)^{n_{2}}}\right] &= 0\\
            \sum_{i=1}^{n_{1}}\frac{(D-i)C_{1}}{(1+y)^{i}} + \frac{(D-n_{1})F_{1}}{(1+y)^{n_{1}}} + \sum_{i=1}^{n_{2}}\frac{(D-i)C_{2}}{(1+y)^{i}} + \frac{(D-n_{2})F_{2}}{(1+y)^{n_{2}}} &= 0\\
            \sum_{i=1}^{n_{1}}\left[\frac{C_{1}D}{(1+y)^i}-\frac{C_{1}i}{(1+y)^{i}}\right]+\frac{F_{1}D}{(1+y)^{n_{1}}}-\frac{F_{1}n_{2}}{(1+y)^{n_{1}}} \\+ \sum_{i=1}^{n_{2}}\left[\frac{C_{2}D}{(1+y)^i}-\frac{C_{2}i}{(1+y)^{i}}\right]+\frac{F_{2}D}{(1+y)^{n_{2}}}-\frac{F_{2}n_{2}}{(1+y)^{n_{2}}} &= 0\\
            -\left[\sum_{i=1}^{n_{1}}\frac{C_{1}i}{(1+y)^{i}}+\frac{F_{1}n_{1}}{(1+y)^{n_{1}}}\right] + D \left[\sum_{i=1}^{n_{1}}\frac{C_{1}}{(1+y)^i}+\frac{F_{1}}{(1+y)^{n_{1}}}\right] \\  -\left[\sum_{i=1}^{n_{2}}\frac{C_{2}i}{(1+y)^{i}}+\frac{F_{2}n_{2}}{(1+y)^{n_{2}}}\right] + D \left[\sum_{i=1}^{n_{2}}\frac{C_{2}}{(1+y)^i}+\frac{F_{2}}{(1+y)^{n_{2}}}\right]&= 0\\\

        \end{aligned}
        \label{induction}
    \end{equation}
    Macaulay duration $MD$ of a coupon bond is:
    \begin{equation}
        \label{md}
        MD = \frac{1}{P}\sum_{i=1}^{n}\left[\frac{Ci}{(1+y)^{i}}+\frac{Fn}{(1+y)^{n}}\right]
    \end{equation}
    substitute (\ref{md}) and (\ref{pv}) to (\ref{induction}):
    \begin{equation*}
        \begin{aligned}
            -P_{1}D_{1} + DP_{1} - P_{2}D_{2} + DP_{2}= 0\\
            D(P_{1}+P_{2})=P_{1}D_{1}+P_{2}D_{2}\\
            \frac{P_1}{P_1+P_2}D_{1}
            + \frac{P_2}{P_1+P_2}D_{2} = D
        \end{aligned}
    \end{equation*}
    Write $\frac{P_1}{P_1+P_2}$ as $\omega_{1}$ and $\frac{P_2}{P_1+P_2}$ as $\omega_{2}$:
    \begin{equation*}
        \omega_{1} + \omega_{2} = 1
    \end{equation*}
    \begin{equation*}
        \omega_{1}D_{1}+\omega_{2}D_{2} = D
    \end{equation*}
\end{document}